a working version of web server in Dafny

ironfleet/src/Dafny/Distributed/Impl/WS/Main.i.dfy
@@ -5,31 +5,7 @@ module Main_i {
     import opened Native__Io_s
     import opened WS__WS_s
     
-    lemma lemma_ByteIsValid(b:byte)
-      ensures 0 <= int(b) < 0x100;
-    {
-    }
-    
-    method BytesArrayToCharArray(requestArr:array<byte>) returns (request:array<char>)
-        requires requestArr != null;
-        requires requestArr.Length > 0;
-        ensures request != null;
-        ensures request.Length == requestArr.Length;
-    {
-        var i := 0;
-        var len := requestArr.Length;
-        request := new char[len];
-                
-        while (i < len)
-            
-        {
-            lemma_ByteIsValid(requestArr[i]);
-            request[i] := UShortToChar(uint16(requestArr[i]));
-            i := i + 1;
-        }
-    }
-
-    method MarshallResponse(response:HTTPResponse) returns (responseArr:array<byte>)
+     /*method MarshallResponse(response:HTTPResponse) returns (responseArr:array<byte>)
         requires 1 < |response| < 65536;
         ensures responseArr != null;
         ensures responseArr.Length == |response|;
@@ -44,7 +20,7 @@ module Main_i {
         }
     }
 
-    method SeqToArray(s:seq<char>)  returns (a:array<char>)
+    method CharSeqToCharArray(s:seq<char>)  returns (a:array<char>)
         ensures a != null;
     {
         a := new char[|s|];
@@ -55,71 +31,218 @@ module Main_i {
             i := i + 1;
         }
         
-    }
+    }*/
 
-    method ExtractFileName(req:array<char>) returns (fileName:array<char>)
-        requires req != null;
-        requires req.Length > 14;
-        ensures fileName != null;
-
+    method ByteSeqToByteArray(s:seq<byte>, a:array<byte>)
+        requires a != null;
+        requires |s| <= a.Length;
+        modifies a;
     {
-        fileName := SeqToArray(req[5..req.Length-9]);
-    }
-
-    method FormulateResponse(header:seq<char>, contents:array<char>) returns (response:HTTPResponse)
-        requires contents != null;
-        requires 1 < |header| + contents.Length < 65536
-        ensures 1 < |response| < 65536;
-    {
-        response := header;
-        var i:= 0;
-        while (i < contents.Length)
+        var i := 0;
+        while (i < |s|)
+            invariant i <= a.Length;
         {
-            response := response + [contents[i]];
+            a[i] := s[i];
             i := i + 1;
         }
-        assume false;
+        
     }
 
-    method Main(ghost env:HostEnvironment) returns (exitCode:int)
+
+    lemma lemma_ByteIsValid(b:byte)
+      ensures 0 <= int(b) < 0x100;
+    {
+    }
+    
+    method BytesArrayToCharArray(b:array<byte>, c:array<char>)
+        requires b != null;
+        requires c != null;
+        requires b.Length == c.Length;
+        requires b.Length > 0;
+        modifies c;
+    {
+        var i := 0;
+        while (i < b.Length)
+            invariant i <= b.Length;
+            invariant i <= c.Length;
+        {
+            lemma_ByteIsValid(b[i]);
+            c[i] := UShortToChar(uint16(b[i]));
+            assert i < b.Length;
+            i := i + 1;
+        }
+    }
+
+   function method Uint32ToBytes(u:uint32) : seq<byte>
+        ensures |Uint32ToBytes(u)| == 10;
+    {
+        [byte(0x30 + (u/1000000000)%10),
+         byte(0x30 + (u/ 100000000)%10),
+         byte(0x30 + (u/  10000000)%10),
+         byte(0x30 + (u/   1000000)%10),
+         byte(0x30 + (u/    100000)%10),
+         byte(0x30 + (u/     10000)%10),
+         byte(0x30 + (u/      1000)%10),
+         byte(0x30 + (u/       100)%10),
+         byte(0x30 + (u/        10)%10),
+         byte(0x30 + (u           )%10)]
+
+    }
+
+    method ParseRequest(request:array<byte>, len:int32, fileName:array<byte>) returns (b:bool)
+        requires request != null;
+        requires int(len) <= request.Length;
+        requires fileName != null;
+        requires fileName.Length >= 10;
+        requires fileName.Length >= int(len);
+        modifies fileName;
+    {
+        var minRequestLength := 5;
+
+        // the request should be at least 5 bytes
+        if (len < minRequestLength) {
+            b := false;
+            return;
+        }
+
+        // check for "GET /" at the beginning
+        if (!(request[0] == 0x47 && request[1] == 0x45 && request[2] == 0x54 && request[3] == 0x20 && request[4] == 0x2F)) {
+            b := false;
+            return;
+        }
+        
+        // extract the fileName from the request by searching for the second space
+        var fileNameLen := 0;
+        var i := minRequestLength;
+        while (i < len)
+            invariant fileNameLen >= 0;
+            invariant 0 <= fileNameLen <= i;
+            invariant 0 <= fileNameLen <= len;
+        {
+            // look for the space
+            if (request[i] == 0x20) {
+                fileName[fileNameLen] := 0x00;
+                break;
+            }
+            fileName[fileNameLen] := request[i]; 
+            fileNameLen := fileNameLen + 1;
+            i := i + 1;
+        }
+        assert int(fileNameLen) <= request.Length;
+        
+        b := true;
+        if (fileNameLen == 0) {
+            fileName[0] := 0x69;
+            fileName[1] := 0x6E;
+            fileName[2] := 0x64;
+            fileName[3] := 0x65;
+            fileName[4] := 0x78;
+            fileName[5] := 0x2E;
+            fileName[6] := 0x68;
+            fileName[7] := 0x74;
+            fileName[8] := 0x6D;
+            fileName[9] := 0x00;
+        } 
+    }
+
+    method StringToBytes(str:seq<char>) returns (bytes:seq<byte>)
+        ensures |bytes| == |str|;
+    {
+        var i := 0;
+        bytes := [];
+        while (i < |str|)
+            invariant i <= |str|;
+            invariant |bytes| == i;
+        {
+            bytes := bytes + [byte(CharToUShort(str[i]) % 0x100)];
+            i := i + 1;
+        }
+        assert|bytes| == |str|;
+    }
+
+
+    method FormulateHeader(code:seq<char>, contentLength:uint32)  returns (header:seq<byte>)
+        requires |code| <= 15;
+        ensures |header| <= 60;
+    {
+        var headerTopStr := "HTTP/1.1 " + code + "\nContent-Length:"; 
+        var contentLengthBytes := Uint32ToBytes(contentLength); 
+        var headerTopBytes := StringToBytes(headerTopStr);
+        var headerTailBytes := StringToBytes("\n\n");
+        header := headerTopBytes + contentLengthBytes + headerTailBytes;
+        assert |header| == |headerTopBytes| + |contentLengthBytes| + |headerTailBytes|;
+    }
+    
+
+    method FormulateResponse(header:seq<byte>, contents:array<byte>) returns (response:array<byte>)
+        requires contents != null;
+        requires |header| + contents.Length <= 60+65536
+        ensures response != null;
+        ensures response.Length <= 60+65536;
+    {
+        var len := |header|;
+
+        if (contents != null) {
+            len := len + contents.Length;
+        }
+
+        response := new byte[len];
+        var i:= 0;
+        while (i < |header|)
+        {
+            response[i] := header[i];
+            i := i + 1;
+        }
+
+        if (contents != null) {
+            while (i < len)
+            {
+                response[i] := contents[i-|header|];
+                i := i + 1;
+            }
+
+        }
+    }
+
+    method {:timeLimitMultiplier 3} Main(ghost env:HostEnvironment) returns (exitCode:int)
         requires env != null && env.Valid() && env.ok.ok();
-        //requires env.udp.history() == [];
         requires |env.constants.CommandLineArgs()| >= 2;
         modifies set x:object | true;
         decreases *; decreases *;
     {
-        var length := int32(65536);
-        var l := new TcpListener.New();
+        var maxLength := int32(65536);
+        var l := new TcpListener.New(8080);
         l.Start();
 
-        var port := l.GetPort();
-        var requestArr := new byte[length];
-        var fileContents := new byte[length];
+        var requestArr := new byte[maxLength];
+        var fileNameBytes := new byte[maxLength];
+        var fileName := new char[maxLength];
+        var fileContents := new byte[maxLength];
         
         var ok := true;
-        var req;
+        //var req;
         var res;
 
         while (ok)
             decreases *;
-            invariant l.started;
+            invariant ok ==> l.started;
             invariant ok ==> env != null && env.Valid() && env.ok.ok();
             //invariant ok ==> Get(env.files, ArrayToSeq(req), ArrayToSeq(res));
         {
+            print ("Waiting for the client request\n");
             var client := l.AcceptTcpClient();
             var len, alive := client.Read(requestArr, 0, int32(requestArr.Length));
             
             if (alive) {
-
-                var i:int32 := 0;
-                req := BytesArrayToCharArray(requestArr);
+                var b := ParseRequest(requestArr, len, fileNameBytes);
+                var header;
                 
-                if (len >= 5 && req[..int32(5)] == "GET /") {
-                    var fileName := ExtractFileName(req);
+                if b {
                     
-                    var b := FileStream.FileExists(fileName, env);
-
-                    if b {
+                    BytesArrayToCharArray(fileNameBytes, fileName);
+                    var fileExists := FileStream.FileExists(fileName, env);
+                    print("Filexists: "); print(fileExists); print("\n\n");
+                    if fileExists {
                         var fileLength;
                         ok, fileLength := FileStream.FileLength(fileName, env);
 
@@ -133,31 +256,43 @@ module Main_i {
                             return;
                         }
                     
-                    
-
-                        if (fileLength > length) {
-                            fileLength := length;
+                        if (fileLength > maxLength) {
+                            fileLength := maxLength;
                         }
 
                         ok := f.Read(0, fileContents, 0, fileLength);
-                        var header := GetProtocolVersion() + " " + GetHTTPCode("OK") + LineBreaks();
-                        var responsePartial := BytesArrayToCharArray(fileContents);
 
-                        res :=  FormulateResponse(header, responsePartial);
+                        if (!ok) {
+                            return;
+                        }
+
+                        header := FormulateHeader("200 OK", uint32(fileLength));
+                        res :=  FormulateResponse(header, fileContents);
+                        assert client.open;
+                        alive := client.Write(res, 0, int32(res.Length));
+                        ok := f.Close();
+                        if (!ok) {
+                            return;
+                        }
+
                     } else {
-                        var header := GetProtocolVersion() + " " + GetHTTPCode("Not Found") + LineBreaks();
-                        res := FormulateResponse(header, null);
+                        header := FormulateHeader("404 Not Found", 0);
+                        var fileContentsTemp := StringToBytes("<html><title>Not Found</title><body>Not Found</body></html>");
+                        assert |fileContentsTemp| <= fileContents.Length;
+                        ByteSeqToByteArray(fileContentsTemp, fileContents);
+                        res :=  FormulateResponse(header, fileContents);
+
+                        alive := client.Write(res, 0, int32(res.Length));
                     }
                 } else {
-                    var header := GetProtocolVersion() + " " + GetHTTPCode("Invalid") + LineBreaks();
-                    res := FormulateResponse(header, null);
-                }
-                
-                var responseArr := MarshallResponse(res);
-                
-                alive := client.Write(responseArr, 0, int32(|res|));
-            }
+                    header := FormulateHeader("500 Invalid", 0);
+                    var fileContentsTemp := StringToBytes("<html><title>Invalid Request</title><body>InValid Request</body></html>");
+                    ByteSeqToByteArray(fileContentsTemp, fileContents);
+                    res :=  FormulateResponse(header, fileContents);
 
+                    alive := client.Write(res, 0, int32(res.Length));       
+                }
+            }
             client.Close();
         }
     }
